theories/rec_lang/adequacy.v
@@ -1,0 +1,118 @@
+From iris.proofmode Require Import tactics.
+From iris.program_logic Require Export adequacy weakestpre.
+From iris.algebra Require Import csum excl auth cmra_big_op gmap.
+From refframe.rec_lang Require Import heap lifting.
+From iris.program_logic Require Export language.
+Set Default Proof Using "Type".
+
+Class reclangPreG Σ := PreRecLangG {
+  reclang_pre_invG :> invPreG Σ;
+  reclang_pre_moduleG :> modulePreG rec_event Σ;
+  reclang_heap_fntbl_inG :> inG Σ fntblUR;
+}.
+
+Definition reclangΣ : gFunctors :=
+  #[invΣ; moduleΣ rec_event; GFunctor (constRF fntblUR)].
+
+Instance subG_reclangPreG {Σ} : subG reclangΣ Σ → reclangPreG Σ.
+Proof. solve_inG. Qed.
+
+Definition iris_module (Λ : language) (initial : cfg Λ) : module (Λ.(observation)) := {|
+  m_state := cfg Λ;
+  m_initial := initial;
+  m_step σ e σ' := step σ (option_list e) σ';
+  m_is_ub σ := ∃ e, e ∈ σ.1 ∧ stuck e σ.2;
+|}.
+
+Definition single_event_head_step (Λ : ectxiLanguage) : Prop :=
+  ∀ κs e σ e' σ' efs, head_step (e:=Λ) e σ κs e' σ' efs → κs = option_list (head κs).
+
+Definition single_event_prim_step (Λ : language) : Prop :=
+  ∀ κs e σ e' σ' efs, prim_step (l:=Λ) e σ κs e' σ' efs → κs = option_list (head κs).
+
+Lemma single_event_head_prim_step Λ:
+  single_event_head_step Λ →
+  single_event_prim_step Λ.
+Proof. move => Hev ?????? [*]. by apply: Hev. Qed.
+
+Lemma single_event_step Λ κs σ σ' :
+  single_event_prim_step Λ →
+  step (Λ:=Λ) σ κs σ' → κs = option_list (head κs).
+Proof. move => Hev [*]. subst. by apply: Hev. Qed.
+
+Lemma has_non_ub_trace_nsteps Λ i σ1 κs σ2:
+  single_event_prim_step Λ →
+  has_non_ub_trace (iris_module Λ i) σ1 κs σ2 ↔ ∃ n, nsteps n σ1 κs σ2.
+Proof.
+  move => Hev.
+  split.
+  - elim; eauto using nsteps_refl.
+    move => /= ??????? [??]. eexists _. by econstructor.
+  - move => [n Hsteps].
+    elim: Hsteps; eauto using NUBTraceEnd.
+    move => /= ???? κ????. erewrite (single_event_step _ κ) => //.
+    apply: NUBTraceStep => //=. by erewrite <-(single_event_step _ κ).
+Qed.
+
+Theorem module_adequacy Σ Λ mspec `{!invPreG Σ} `{!modulePreG Λ.(observation) Σ} es σ1:
+  (∀ κs, LEM ((∃ κs' σ, κs' `prefix_of` κs ∧ has_trace mspec mspec.(m_initial) κs' σ ∧ mspec.(m_is_ub) σ))) →
+  single_event_prim_step Λ →
+  (∀ `{Hinv : !invG Σ} γm κsfull,
+       let _ : moduleG Λ.(observation) Σ := ModuleG Λ.(observation) Σ mspec _ γm κsfull in
+     ⊢ spec_ctx κsfull -∗
+       own_module Λ.(observation) module_spec_name mspec mspec.(m_initial) ={⊤}=∗
+       ∃ (stateI : state Λ → list (observation Λ) → nat → iProp Σ)
+         (fork_post : val Λ → iProp Σ),
+       let _ : irisG Λ Σ := IrisG _ _ Hinv stateI fork_post in
+       stateI σ1 κsfull 0 ∗
+       ([∗ list] e ∈ es, WP e @ ⊤ {{ _, True }}) ∗
+       (∀ σ2 n, stateI σ2 [] n ={⊤,∅}=∗ spec_ctx [])) →
+  refines (iris_module Λ (es, σ1)) mspec.
+Proof.
+  move => HLEM Hev /= Hwp.
+  apply: refines_assume_non_ub => // κsfull σ2 Htrace Hnoub.
+  move: Htrace => /has_trace_to_non_ub_trace[κs' [[??] [? [Htrace Hor]]]].
+  move: Htrace => /has_non_ub_trace_nsteps[//|?] /=.
+  apply: wp_strong_adequacy => ?.
+  iMod (ghost_var_alloc (ModState mspec mspec.(m_initial))) as (γm) "[Hm1 Hm2]".
+  iMod (Hwp _ γm κs' with "[Hm1] Hm2") as (stateI fork_post) "(Hσ&Hwp&Hend)". {
+    iExists [], _. iFrame. iPureIntro. split_and! => //. { by constructor. }
+    move => ? /= [? Hκs']. subst. apply: Hnoub. etrans. 2: done. eexists _. by rewrite fmap_app.
+  }
+  iModIntro. iExists NotStuck, stateI, (replicate (length es) (λ _, True%I)), fork_post.
+  rewrite big_sepL2_replicate_r //. iFrame.
+  iIntros (es' ts' ?? Hnonstuck) "Hs _ _".
+  iMod ("Hend" with "Hs") as (κs σscur Hmodful Htrace _) "_". iPureIntro.
+  rewrite app_nil_r in Hmodful. simpl in *. subst.
+  case: Hor => [[<- ?]|[? [? /not_not_stuck Hstuck]]]; naive_solver.
+Qed.
+
+
+
+Lemma reclang_adequacy Σ `{!reclangPreG Σ} mspec (mains : list lang.expr) (fns : gmap fn_name fndef):
+  (∀ κs, LEM ((∃ κs' σ, κs' `prefix_of` κs ∧ has_trace mspec mspec.(m_initial) κs' σ ∧ mspec.(m_is_ub) σ))) →
+  (∀ {HrecG : reclangG Σ},
+    ⊢ @own_module _ rec_event (module_ghostvarG) module_spec_name mspec mspec.(m_initial) -∗
+      fntbl fns
+      ={⊤}=∗ [∗ list] main ∈ mains, WP main {{ _, True }}) →
+  refines (iris_module rec_lang (mains, {| st_fns := fns |})) mspec.
+Proof.
+  move => HLEM Hwp. apply: module_adequacy; [done| | ]. {
+    apply: single_event_head_prim_step.
+    move => ??????. by inversion 1.
+  }
+  iIntros (Hinv γm κsfull Hmod) "Hs Hm".
+  (* set h := to_heap ∅. *)
+  (* iMod (own_alloc (● h ⋅ ◯ h)) as (γh) "[Hh _]" => //. *)
+  (* { apply auth_both_valid_discrete. split => //. } *)
+  set f := to_fntbl fns.
+  iMod (own_alloc (f)) as (γf) "Hf" => //.
+
+  set (HheapG := HeapG _ _ γf Hmod).
+  set (HreclangG := RecLangG _ _ HheapG).
+  iAssert (fntbl fns) as "#Hfns". { by rewrite fntbl_eq. }
+  iMod (Hwp HreclangG with "Hm Hfns") as "Hes".
+  iModIntro. iExists _, _. iFrame "Hes Hs Hfns".
+  iIntros (??) "[? Hσ]". iFrame.
+  by iMod (fupd_intro_mask' _ ∅).
+Qed.
