theories/rec_lang/examples.v
@@ -1,0 +1,76 @@
+From refframe.rec_lang Require Export proofmode.
+From refframe.rec_lang Require Import adequacy.
+
+Section examples.
+Context `{!reclangG Σ}.
+
+Inductive test_state : Type :=
+| TSInit | TSCall (n : Z) | TSFinal | TSUb.
+Inductive test_step : test_state → option rec_event → test_state → Prop :=
+| TSSInit n:
+  test_step TSInit (Some $ CallEvt "extfn" [ValNum n]) (TSCall n)
+| TSSCall n v:
+  test_step (TSCall n) (Some $ RecvRetEvt v) (if bool_decide (v = n) then TSFinal else TSUb).
+Definition test_module : module rec_event := {|
+  m_state := test_state;
+  m_initial := TSInit;
+  m_step := test_step;
+  m_is_ub σ := σ = TSUb;
+|}.
+
+Definition test_main : lang.expr :=
+  LetE "n" (BinOp 1 AddOp 1) $
+  LetE "ret" (Call "extfn" [ Var "n" ] ) $
+  BinOp (Var "ret") EqOp 2.
+
+Lemma wp_test_main :
+  fntbl_entry "extfn" None -∗
+  own_module rec_event module_spec_name test_module TSInit -∗
+  WP test_main {{ v, ⌜v = 1⌝ }}.
+Proof.
+  iIntros "#Hextfn Hm".
+  rewrite /test_main.
+  iStartProof.
+  wp_bind (BinOp _ _ _).
+  iApply wp_binop. iModIntro.
+  iApply wp_let. simpl. iModIntro.
+  wp_bind (Call _ _).
+  iApply (wp_ext_call [_]) => //.
+
+  iExists test_module.
+  iMod (fupd_intro_mask' _ ∅) as "HE" => //. do 2 iModIntro.
+  iExists _. iFrame "Hm".
+  iExists _. iSplit. { iPureIntro. apply: TraceStepSome. econstructor. constructor. }
+  iIntros "Hm" (_). iMod "HE" as %_.
+  iIntros "!>" (v).
+
+  iExists test_module.
+  iMod (fupd_intro_mask' _ ∅) as "HE" => //. do 2 iModIntro.
+  iExists _. iFrame "Hm".
+  iExists _. iSplit. { iPureIntro. apply: TraceStepSome. econstructor. constructor. }
+  iIntros "Hm" (Hub). iMod "HE" as %_.
+  case_bool_decide; subst. 2: {
+    contradict Hub. eexists _. apply: TraceStepSome. econstructor.
+    econstructor. by case_bool_decide.
+  }
+  iIntros "!>".
+
+  iApply wp_let => /=. iModIntro.
+  iApply wp_binop. iPureIntro. by case_bool_decide.
+  Unshelve.
+  apply: TSInit.
+Qed.
+
+End examples.
+
+Lemma test_main_adequate :
+  (∀ κs, LEM ((∃ κs' σ, κs' `prefix_of` κs ∧ has_trace test_module test_module.(m_initial) κs' σ ∧ test_module.(m_is_ub) σ))) →
+  refines (iris_module rec_lang ([test_main], {| st_fns := ∅ |})) test_module.
+Proof.
+  move => HLEM.
+  set Σ : gFunctors := #[reclangΣ].
+  apply: (reclang_adequacy Σ) => //.
+  iIntros (?) "Hown #Hfn /=". iModIntro. iSplitL => //.
+  iApply wp_mono. by iIntros (?) "_".
+  iApply wp_test_main => //. by iApply (fntbl_entry_intro with "Hfn").
+Qed.
