theories/rec_lang/heap.v
@@ -1,0 +1,124 @@
+From iris.proofmode Require Import tactics.
+From iris.program_logic Require Export weakestpre.
+From stdpp Require Import coPset.
+From iris.algebra Require Import big_op gmap frac agree.
+From iris.algebra Require Import csum excl auth cmra_big_op numbers.
+From iris.bi Require Import fractional.
+From iris.base_logic Require Export lib.own lib.ghost_var.
+Require Import refframe.rec_lang.lang.
+
+Definition fntblUR : cmra :=
+  agreeR (gmapO fn_name fndefO).
+
+Record mod_state EV := ModState {
+  ms_module : module EV;
+  ms_state : ms_module.(m_state);
+}.
+Arguments ModState {_}.
+Arguments ms_module {_}.
+Arguments ms_state {_}.
+
+Class moduleG EV Σ := ModuleG {
+  module_spec : module EV;
+  module_ghostvarG :> ghost_varG Σ (mod_state EV);
+  module_spec_name : gname;
+  module_full_trace : list EV;
+}.
+
+Class modulePreG EV Σ := PreModuleG {
+  module_pre_ghostvarG :> ghost_varG Σ (mod_state EV);
+}.
+
+Definition moduleΣ EV : gFunctors :=
+  #[ghost_varΣ (mod_state EV)].
+
+Instance subG_modulePreG {Σ} EV : subG (moduleΣ EV) Σ → modulePreG EV Σ.
+Proof. solve_inG. Qed.
+
+Definition own_module {Σ} EV `{!ghost_varG Σ (mod_state EV)} (γ : gname) (m : module EV) (σ : m.(m_state)) :=
+  ghost_var γ (1/2) (ModState m σ).
+Definition WPspec {Σ} EV `{!ghost_varG Σ (mod_state EV)} `{!invG Σ} (γ : gname) (κs : list EV) (E : coPset) (Φ : iProp Σ) : iProp Σ :=
+  |={E, ∅}=> ▷ ∃ m σ, own_module EV γ m σ ∗
+   ∃ σ', ⌜has_trace m σ (Vis <$> κs) σ'⌝ ∗ (
+         own_module EV γ m σ' -∗
+        ⌜¬ ∃ σub, has_trace m σ ((Vis <$> κs) ++ [Ub]) σub⌝ -∗
+        |={∅, E}=> Φ).
+
+
+Class heapG Σ := HeapG {
+  heap_fntbl_inG :> inG Σ (fntblUR);
+  heap_fntbl_name : gname;
+  heap_module :> moduleG rec_event Σ;
+}.
+
+Section definitions.
+  Context `{!moduleG EV Σ}.
+
+  Definition spec_ctx (κsrest : list EV) : iProp Σ :=
+    ∃ κsstart σscur,
+      ⌜module_full_trace = κsstart ++ κsrest⌝ ∗
+      ⌜has_trace module_spec module_spec.(m_initial) (Vis <$> κsstart) σscur⌝ ∗
+      (* obtained by classical reasoning before switching to Iris *)
+      ⌜∀ κs, κs `prefix_of` module_full_trace → ¬ ∃ σub, has_trace module_spec module_spec.(m_initial) ((Vis <$>  κs) ++ [Ub]) σub⌝ ∗
+      own_module EV module_spec_name module_spec σscur.
+
+End definitions.
+
+Definition to_fntbl : gmap fn_name fndef → fntblUR :=
+  to_agree.
+
+Section definitions.
+  Context `{!heapG Σ}.
+
+  Definition fntbl_def (fns : gmap fn_name fndef) : iProp Σ :=
+    own heap_fntbl_name (to_fntbl fns).
+  Definition fntbl_aux : seal (@fntbl_def). by eexists. Qed.
+  Definition fntbl := unseal fntbl_aux.
+  Definition fntbl_eq : @fntbl = @fntbl_def :=
+    seal_eq fntbl_aux.
+
+  Definition fntbl_entry_def (l : fn_name) (f: option fndef) : iProp Σ :=
+    ∃ fns, ⌜fns !! l = f⌝ ∗ fntbl fns.
+  Definition fntbl_entry_aux : seal (@fntbl_entry_def). by eexists. Qed.
+  Definition fntbl_entry := unseal fntbl_entry_aux.
+  Definition fntbl_entry_eq : @fntbl_entry = @fntbl_entry_def :=
+    seal_eq fntbl_entry_aux.
+
+  Definition state_ctx (σ: rec_state) (κs : list rec_event) : iProp Σ :=
+    fntbl σ.(st_fns) ∗ spec_ctx κs.
+End definitions.
+
+Section fntbl.
+  Context `{!heapG Σ}.
+
+  Lemma to_fntbl_valid f : ✓ to_fntbl f.
+  Proof. done. Qed.
+
+  Global Instance fntbl_pers fns : Persistent (fntbl fns).
+  Proof. rewrite fntbl_eq. by apply _. Qed.
+
+  Global Instance fntbl_entry_pers f fn : Persistent (fntbl_entry f fn).
+  Proof. rewrite fntbl_entry_eq. by apply _. Qed.
+
+  Lemma fntbl_agree fns1 fns2 :
+    fntbl fns1 -∗ fntbl fns2 -∗ ⌜fns1 = fns2⌝.
+  Proof.
+    rewrite fntbl_eq. iIntros "H1 H2".
+    iDestruct (own_valid_2 with "H1 H2") as %?%to_agree_op_valid.
+      by fold_leibniz.
+  Qed.
+
+  Lemma fntbl_entry_intro t f fn :
+    t !! f = fn →
+    fntbl t -∗ fntbl_entry f fn.
+  Proof. rewrite fntbl_entry_eq. iIntros (?) "?". iExists _. by iFrame. Qed.
+
+  Lemma fntbl_entry_lookup t f fn :
+    fntbl t -∗ fntbl_entry f fn -∗ ⌜t !! f = fn⌝.
+  Proof.
+    rewrite fntbl_entry_eq. iIntros "Htbl Hf".
+    iDestruct "Hf" as (fns2 ?) "Hf".
+    by iDestruct (fntbl_agree with "Htbl Hf") as %->.
+  Qed.
+
+End fntbl.
