theories/rec_lang/lang.v
@@ -1,0 +1,185 @@
+Require Import stdpp.strings.
+Require Import stdpp.propset.
+From iris.program_logic Require Export language ectx_language ectxi_language.
+Require Export refframe.base.
+Require Export refframe.module.
+
+Definition fn_name := string.
+Definition var_name := string.
+
+Inductive binop : Set :=
+| AddOp | EqOp.
+
+Inductive val := | ValNum (z : Z).
+Coercion ValNum : Z >-> val.
+Global Instance val_eq_dec : EqDecision val.
+Proof. solve_decision. Qed.
+
+Inductive expr : Set :=
+| Var (v : var_name)
+| Val (v : val)
+| BinOp (e1 : expr) (o : binop) (e2 : expr)
+| If (e e1 e2 : expr)
+| LetE (v : var_name) (e1 e2 : expr)
+| Call (f : fn_name) (args : list expr)
+| Waiting
+.
+Coercion Val : val >-> expr.
+
+Fixpoint subst (x : var_name) (v : val) (e : expr) : expr :=
+  match e with
+  | Var y => if bool_decide (x = y) then Val v else Var y
+  | Val v => Val v
+  | BinOp e1 o e2 => BinOp (subst x v e1) o (subst x v e2)
+  | If e e1 e2 => If (subst x v e) (subst x v e1) (subst x v e2)
+  | LetE y e1 e2 => LetE y (subst x v e1) (if bool_decide (x ≠ y) then subst x v e2 else e2)
+  | Call f args => Call f (subst x v <$> args)
+  | Waiting => Waiting
+  end.
+Fixpoint subst_l (xs : list var_name) (vs : list val) (e : expr) : expr :=
+  match xs, vs with
+  | x::xs', v::vs' => subst_l xs' vs' (subst x v e)
+  | _,_ => e
+  end.
+
+Inductive expr_ectx :=
+| BinOpLCtx (op : binop) (e2 : expr)
+| BinOpRCtx (v1 : val) (op : binop)
+| IfCtx (e2 e3 : expr)
+| LetECtx (v : var_name) (e2 : expr)
+| CallCtx (f : fn_name) (vl : list val) (el : list expr)
+.
+
+Definition expr_fill_item (Ki : expr_ectx) (e : expr) : expr :=
+  match Ki with
+  | BinOpLCtx op e2 => BinOp e op e2
+  | BinOpRCtx v1 op => BinOp v1 op e
+  | IfCtx e2 e3 => If e e2 e3
+  | LetECtx v e2 => LetE v e e2
+  | CallCtx f vl el => Call f ((Val <$> vl) ++ e :: el)
+  end.
+
+Record fndef : Type := {
+  fd_args : list var_name;
+  fd_body : expr;
+}.
+
+Record rec_state := {
+  st_fns : gmap fn_name fndef;
+}.
+
+Inductive rec_event : Type :=
+| RecvCallEvt (fn : fn_name) (args: list val) | RecvRetEvt (ret: val)
+| CallEvt (fn : fn_name) (args: list val) | DoneEvt (ret: val).
+
+Inductive step : expr → rec_state → list rec_event → expr → rec_state → list expr → Prop :=
+| BinOpStep n1 op n2 σ:
+    step (BinOp (Val (ValNum n1)) op (Val (ValNum n2))) σ []
+         (match op with | AddOp => n1 + n2 | EqOp => Z_of_bool $ bool_decide (n1 = n2) end%Z) σ []
+| IfStep n e1 e2 σ:
+    step (If (Val (ValNum n)) e1 e2) σ [] (if bool_decide (n ≠ 0) then e1 else e2) σ []
+| LetStep x v e σ:
+    step (LetE x (Val v) e) σ [] (subst x v e) σ []
+| CallInternalStep f fn σ vs:
+    σ.(st_fns) !! f = Some fn →
+    length vs = length fn.(fd_args) →
+    step (Call f (Val <$> vs)) σ [] (subst_l fn.(fd_args) vs fn.(fd_body)) σ []
+| CallExternalStep f σ vs:
+    σ.(st_fns) !! f = None →
+    step (Call f (Val <$> vs)) σ [CallEvt f vs] Waiting σ []
+| RecvReturnStep σ v:
+    step Waiting σ [RecvRetEvt v] (Val v)  σ []
+(* (* External Calls *) *)
+(* | CallExternalStep f vas ρ cs fns nas: *)
+(*     Forall2 (λ n v, ρ !! n = Some v) vas nas → *)
+(*     fns !! f = None → *)
+(*     step {| st_exp := Running (Call f vas); st_env := ρ; st_conts := cs; st_fns := fns |} *)
+(*          (Some (CallEvt f nas)) *)
+(*          {| st_exp := WaitingForReturn; st_env := ρ; st_conts := cs; st_fns := fns |} *)
+(* | RecvReturnStep ρ cs fns n: *)
+(*     step {| st_exp := WaitingForReturn; st_env := ρ; st_conts := cs; st_fns := fns |} *)
+(*          (Some (RecvRetEvt n)) *)
+(*          {| st_exp := Running (Const n); st_env := ρ; st_conts := cs; st_fns := fns |} *)
+(* | RecvCallStep ρ cs fns nas σ fn f: *)
+(*     fns !! f = Some fn → *)
+(*     σ = (if bool_decide (length nas = length fn.(fd_args)) then Running fn.(fd_body) else Stuck) → *)
+(*     step {| st_exp := WaitingForCall; st_env := ρ; st_conts := cs; st_fns := fns |} *)
+(*          (Some (RecvCallEvt f nas)) *)
+(*          {| st_exp := σ; st_env := list_to_map (zip fn.(fd_args) nas); st_conts := cs; st_fns := fns |} *)
+(* (* Const steps *) *)
+(* | ConstConsStep n c ρ fns cs: *)
+(*     step {| st_exp := Running (Const n); st_env := ρ; st_conts := c::cs; st_fns := fns |} *)
+(*          None *)
+(*          {| st_exp := Running c.(c_expr); st_env := <[c.(c_var) := n]>c.(c_env); st_conts := cs; st_fns := fns |} *)
+(* | ConstNilStep n ρ fns: *)
+(*     step {| st_exp := Running (Const n); st_env := ρ; st_conts := []; st_fns := fns |} *)
+(*          (Some (DoneEvt n)) *)
+(*          {| st_exp := Finished; st_env := ρ; st_conts := []; st_fns := fns |} *)
+(* . *).
+
+
+
+Definition to_val (e : expr) : option val := if e is Val v then Some v else None.
+Definition of_val (v : val) : expr := Val v.
+
+Lemma list_expr_val_eq_inv vl1 vl2 e1 e2 el1 el2 :
+  (Val <$> vl1) ++ e1 :: el1 = (Val <$> vl2) ++ e2 :: el2 →
+  to_val e1 = None → to_val e2 = None →
+  vl1 = vl2 ∧ e1 = e2 ∧ el1 = el2.
+Proof.
+  revert vl2; induction vl1; destruct vl2; inversion 1; intros He1 He2.
+  - done.
+  - subst. by inversion He1.
+  - subst. by inversion He2.
+  - destruct (IHvl1 vl2); auto. split; f_equal; auto.
+Qed.
+Lemma list_expr_val_eq_false vl1 vl2 e el :
+  to_val e = None → Val <$> vl1 = (Val <$> vl2) ++ e :: el → False.
+Proof.
+  move => He. elim: vl2 vl1 => [[]//=*|v vl2 IH [|??]?]; csimpl in *; simplify_eq; eauto.
+Qed.
+
+
+Lemma of_to_val e v : to_val e = Some v → of_val v = e.
+Proof. case: e => //. naive_solver. Qed.
+
+Lemma val_stuck e1 σ1 κ e2 σ2 ef :
+  step e1 σ1 κ e2 σ2 ef → to_val e1 = None.
+Proof. destruct 1 => //. Qed.
+
+Instance fill_item_inj Ki : Inj (=) (=) (expr_fill_item Ki).
+Proof. destruct Ki; intros ???; simplify_eq/=; auto with f_equal. Qed.
+
+Lemma fill_item_val Ki e :
+  is_Some (to_val (expr_fill_item Ki e)) → is_Some (to_val e).
+Proof. intros [v ?]. destruct Ki; simplify_option_eq; eauto. Qed.
+
+Lemma fill_item_no_val_inj Ki1 Ki2 e1 e2 :
+  to_val e1 = None → to_val e2 = None →
+  expr_fill_item Ki1 e1 = expr_fill_item Ki2 e2 → Ki1 = Ki2.
+Proof.
+  move: Ki1 Ki2 => [ ^ Ki1] [ ^Ki2] He1 He2 HEQ //; simplify_eq => //.
+  efeed pose proof list_expr_val_eq_inv => //. naive_solver.
+Qed.
+
+Lemma expr_ctx_step_val Ki e σ1 κ e2 σ2 ef :
+  step (expr_fill_item Ki e) σ1 κ e2 σ2 ef → is_Some (to_val e).
+Proof.
+  destruct Ki; inversion 1; simplify_eq/=; eauto.
+  all: apply not_eq_None_Some; intros ?; by eapply list_expr_val_eq_false.
+Qed.
+
+Lemma rec_lang_mixin : EctxiLanguageMixin of_val to_val expr_fill_item step.
+Proof.
+  split => //; eauto using of_to_val, val_stuck, fill_item_inj, fill_item_val, fill_item_no_val_inj, expr_ctx_step_val.
+Qed.
+Canonical Structure rec_ectxi_lang := EctxiLanguage rec_lang_mixin.
+Canonical Structure rec_ectx_lang := EctxLanguageOfEctxi rec_ectxi_lang.
+Canonical Structure rec_lang := LanguageOfEctx rec_ectx_lang.
+
+Instance val_inhabited : Inhabited val := populate $ ValNum 1.
+Instance expr_inhabited : Inhabited expr := populate (Val inhabitant).
+Instance fndef_inhabited : Inhabited fndef := populate {| fd_args := []; fd_body := inhabitant |}.
+Instance state_inhabited : Inhabited rec_state := populate {| st_fns := inhabitant |}.
+
+Canonical Structure fndefO := leibnizO fndef.
