theories/rec_lang/lifting.v
@@ -1,0 +1,98 @@
+From iris.proofmode Require Import tactics.
+From iris.program_logic Require Export weakestpre.
+From iris.program_logic Require Import ectx_lifting.
+From refframe.rec_lang Require Export lang heap.
+Set Default Proof Using "Type".
+Import uPred.
+
+Class reclangG Σ := RecLangG {
+  rec_lang_invG : invG Σ;
+  rec_lang_gen_heapG :> heapG Σ
+}.
+
+Instance rec_irisG `{!reclangG Σ} : irisG rec_lang Σ := {
+  iris_invG := rec_lang_invG;
+  state_interp σ κs _ := state_ctx σ κs;
+  fork_post _ := True%I;
+}.
+Global Opaque iris_invG.
+
+Local Hint Extern 0 (reducible _ _) => eexists _, _, _, _; simpl : core.
+Local Hint Extern 0 (head_reducible _ _) => eexists _, _, _, _; simpl : core.
+
+Section lifting.
+Context `{!reclangG Σ}.
+
+Lemma wp_binop Φ (n1 n2 : Z) op E:
+  ▷ Φ (ValNum (match op with | AddOp => n1 + n2 | EqOp => Z_of_bool (bool_decide (n1 = n2)) end))%Z -∗
+  WP BinOp (Val n1) op (Val n2) @ E {{ Φ }}.
+Proof.
+  iIntros "HΦ".
+  iApply wp_lift_atomic_head_step_no_fork; auto.
+  iIntros (σ1 κ κs n) "Hctx !>".
+  iSplit; first by eauto using BinOpStep.
+  iIntros "!# /=" (e2 σ2 efs Hst). invert_all lang.step.
+  iModIntro. iFrame. iSplit => //. by case_match.
+Qed.
+
+Lemma wp_let E Φ n v e:
+  ▷ WP (subst n v e) @ E {{ Φ }} -∗
+  WP LetE n (Val v) e @ E {{ Φ }}.
+Proof.
+  iIntros "HΦ".
+  iApply wp_lift_pure_det_head_step_no_fork'; eauto using LetStep.
+  move => /= *. invert_all lang.step. naive_solver.
+Qed.
+
+Lemma wp_if E Φ e1 e2 n:
+  ▷ WP (if bool_decide (n ≠ 0) then e1 else e2) @ E {{ Φ }} -∗
+  WP If (Val n) e1 e2 @ E {{ Φ }}.
+Proof.
+  iIntros "HΦ".
+  iApply wp_lift_pure_det_head_step_no_fork'; eauto using IfStep.
+  move => /= *. invert_all lang.step. do 2 case_bool_decide; naive_solver.
+Qed.
+
+Lemma wp_call E Φ f vs fn:
+  length vs = length fn.(fd_args) →
+  fntbl_entry f (Some fn) -∗
+  ▷ WP (subst_l fn.(fd_args) vs fn.(fd_body)) @ E {{ Φ }} -∗
+  WP Call f (Val <$> vs) @ E {{ Φ }}.
+Proof.
+  iIntros (?) "Hfn HΦ".
+  iApply wp_lift_head_step; auto.
+  iIntros (σ1 κ κs n) "(Hfctx & Hsctx)".
+  iDestruct (fntbl_entry_lookup with "Hfctx Hfn") as %?.
+  iMod (fupd_intro_mask' _ ∅) as "HE". set_solver.
+  iModIntro.
+  iSplit; first by eauto using CallInternalStep.
+  iIntros "!# /=" (e2 σ2 efs Hst). iMod "HE". invert_all lang.step.
+  iModIntro. iFrame.
+Qed.
+
+Lemma wp_ext_call vs E Φ f:
+  fntbl_entry f None -∗
+  WPspec rec_event module_spec_name [CallEvt f vs] E (∀ v, WPspec rec_event module_spec_name [RecvRetEvt v] E (Φ v))  -∗
+  WP Call f (Val <$> vs) @ E {{ Φ }}.
+Proof.
+  iIntros "Hfn HΦ".
+  iApply wp_lift_head_step; auto.
+  iIntros (σ1 κ κs n) "(Hfctx & Hsctx)".
+  iDestruct (fntbl_entry_lookup with "Hfctx Hfn") as %?.
+  iMod "HΦ". iModIntro.
+  iSplit; first by eauto using CallExternalStep.
+  iIntros "!# /=" (e2 σ2 efs Hst). invert_all lang.step.
+
+  iDestruct "HΦ" as (??) "[Hm HΦ]".
+  iDestruct "Hsctx" as (?????) "Hm2".
+  iDestruct (ghost_var_agree with "Hm Hm2") as %Heq.
+  Require Import Coq.Program.Equality.
+  dependent destruction Heq.
+  iDestruct "HΦ" as (? ?) "HΦ".
+  iMod (ghost_var_update_halves with "Hm Hm2") as "[Hm Hm2]".
+  iMod ("HΦ" with "Hm [%]") as "HΦ". admit.
+Admitted.
+
+
+
+End lifting.
