theories/rec_lang/proofmode.v
@@ -1,0 +1,46 @@
+From iris.proofmode Require Import coq_tactics reduction.
+From iris.proofmode Require Export tactics.
+From iris.program_logic Require Import atomic.
+From refframe.rec_lang Require Export lifting.
+From iris.prelude Require Import options.
+
+
+(** The tactic [reshape_expr e tac] decomposes the expression [e] into an
+evaluation context [K] and a subexpression [e']. It calls the tactic [tac K e']
+for each possible decomposition until [tac] succeeds. *)
+Ltac reshape_expr e tac :=
+  (* Note that the current context is spread into a list of fully-constructed
+     items [K] A fully-constructed item is inserted into [K] by calling
+     [add_item]. *)
+  let rec go K e :=
+    match e with
+    | _                               => tac K e
+    | BinOp ?op ?e (Val ?v)           => add_item (BinOpLCtx op v) K e
+    | BinOp ?op ?e1 ?e2               => add_item (BinOpRCtx op e1) K e2
+    | If ?e0 ?e1 ?e2                  => add_item (IfCtx e1 e2) K e0
+    | LetE ?v ?e1 ?e2                 => add_item (LetECtx v e2) K e1
+    end
+  with add_item Ki K e := go (Ki :: K) e
+  in go (@nil expr_ectx) e.
+
+
+Lemma tac_wp_bind `{!reclangG Σ} K Δ s E Φ e f :
+  f = (λ e, fill K e) → (* as an eta expanded hypothesis so that we can `simpl` it *)
+  envs_entails Δ (WP e @ s; E {{ v, WP f (Val v) @ s; E {{ Φ }} }})%I →
+  envs_entails Δ (WP fill K e @ s; E {{ Φ }}).
+Proof. rewrite envs_entails_eq=> -> ->. by apply: wp_bind. Qed.
+
+Ltac wp_bind_core K :=
+  lazymatch eval hnf in K with
+  | [] => idtac
+  | _ => eapply (tac_wp_bind K); [simpl; reflexivity|reduction.pm_prettify]
+  end.
+
+Tactic Notation "wp_bind" open_constr(efoc) :=
+  iStartProof;
+  lazymatch goal with
+  | |- envs_entails _ (wp ?s ?E ?e ?Q) =>
+    first [ reshape_expr e ltac:(fun K e' => unify e' efoc; wp_bind_core K)
+          | fail "wp_bind: cannot find" efoc "in" e ]
+  | _ => fail "wp_bind: not a 'wp'"
+  end.
